Verified Bedrock module with all the methods Ben enumerated originally for Fiat examples (plus 'delete' for finite sets)

platform/facade/examples/FiatImpl.v
@@ -10,7 +10,7 @@ Require Import Cito.RepInv Cito.MakeADT.
 
 Require Import AutoSep.
 
-Require Import ListSetF FiatRepInv.
+Require Import ListSetF ListSeqF FiatRepInv.
 
 Module Import Made := MakeADT.Make(FiatADTs.Adt)(Ri).
 
@@ -36,6 +36,33 @@ Lemma readd_FEnsemble : forall c rv rv',
   intros.
   unfold is_heap at 2.
   assert (List.In (c, FEnsemble rv') (heap_elements (WordMap.add c (FEnsemble rv') (heap_upd heap_empty c (FEnsemble rv))))).
+  Import LayoutHintsUtil.
+  apply InA_In.
+  apply WordMap.elements_1.
+  apply WordMap.add_1.
+  auto.
+  eapply starL_in in H; try (apply NoDupA_NoDup; apply WordMap.elements_3w).
+  destruct H; intuition idtac.
+  eapply Himp_trans; [ | apply H0 ].
+  simpl.
+  apply Himp_star_frame; try apply Himp_refl.
+  apply starL_permute; auto.
+  apply NoDupA_NoDup; apply WordMap.elements_3w.
+  intuition.
+  apply H2 in H1; intuition.
+  apply In_InA' in H4.
+  apply WordMap.elements_2 in H4.
+  apply Properties.F.add_mapsto_iff in H4; intuition.
+  apply Properties.F.add_mapsto_iff in H5; intuition.
+  apply Properties.F.empty_mapsto_iff in H6; tauto.
+Qed.
+
+Lemma readd_List : forall c rv rv',
+  lseq rv' c * is_heap heap_empty
+  ===> is_heap (WordMap.add c (List rv') (heap_upd heap_empty c (List rv))).
+  intros.
+  unfold is_heap at 2.
+  assert (List.In (c, List rv') (heap_elements (WordMap.add c (List rv') (heap_upd heap_empty c (List rv))))).
   Import LayoutHintsUtil.
   apply InA_In.
   apply WordMap.elements_1.
@@ -144,12 +171,20 @@ Require AxSpec.
 Import AxSpec.ConformTactic.
 
 Definition m0 := bimport [[ "sys"!"abort" @ [abortS],
+
                             "ListSet"!"new" @ [ListSetF.newS],
                             "ListSet"!"delete" @ [ListSetF.deleteS],
                             "ListSet"!"mem" @ [ListSetF.memS],
                             "ListSet"!"add" @ [ListSetF.addS],
                             "ListSet"!"remove" @ [ListSetF.removeS],
-                            "ListSet"!"size" @ [ListSetF.sizeS] ]]
+                            "ListSet"!"size" @ [ListSetF.sizeS],
+
+                            "ListSeq"!"new" @ [ListSeqF.newS],
+                            "ListSeq"!"delete" @ [ListSeqF.deleteS],
+                            "ListSeq"!"pop" @ [ListSeqF.popS],
+                            "ListSeq"!"empty" @ [ListSeqF.emptyS],
+                            "ListSeq"!"push" @ [ListSeqF.pushS],
+                            "ListSeq"!"copy" @ [ListSeqF.copyS] ]]
   fmodule "ADT" {{
     ffunction "sEmpty" reserving 8 [FEnsemble_sEmpty] := "ListSet"!"new"
     with ffunction "sDelete" reserving 7 [FEnsemble_sDelete] := "ListSet"!"delete"
@@ -157,6 +192,12 @@ Definition m0 := bimport [[ "sys"!"abort" @ [abortS],
     with ffunction "sRemove" reserving 7 [FEnsemble_sRemove] := "ListSet"!"remove"
     with ffunction "sIn" reserving 1 [FEnsemble_sIn] := "ListSet"!"mem"
     with ffunction "sSize" reserving 1 [FEnsemble_sSize] := "ListSet"!"size"
+    with ffunction "new" reserving 8 [List_new] := "ListSeq"!"new"
+    with ffunction "delete" reserving 7 [List_delete] := "ListSeq"!"delete"
+    with ffunction "pop" reserving 8 [List_pop] := "ListSeq"!"pop"
+    with ffunction "empty" reserving 0 [List_empty] := "ListSeq"!"empty"
+    with ffunction "push" reserving 8 [List_push] := "ListSeq"!"push"
+    with ffunction "copy" reserving 10 [List_copy] := "ListSeq"!"copy"
   }}.
 
 Theorem ok0 : moduleOk m0.
@@ -297,7 +338,133 @@ Theorem ok0 : moduleOk m0.
   do_delegate2 ("self" :: nil).
 
 
+  (* ListSeq *)
+
+  (* new *)
+
+  do_abort (@nil string).
+  do_abort (@nil string).
+  do_abort (@nil string).
+
+  do_delegate1 (@nil string) hints.
+  do 2 (descend; step auto_ext).
+  2: returnAdt.
+  simpl.
+  make_toArray (@nil string).
+  step auto_ext.
+  etransitivity; [ | apply himp_star_frame; [ apply (@is_state_in x4) | reflexivity ] ].
+  unfolder.
+  do_delegate2 (@nil string).
+
+  (* delete *)
+  
+  do_abort ("self" :: nil).
+  do_abort ("self" :: nil).
+  do_abort ("self" :: nil).
+
+  do_delegate1 ("self" :: nil) hints.
+  descend; step auto_ext.
+  repeat (apply andL || (apply injL; intro) || (apply existsL; intro)); reduce.
+  apply get_rval''; intro.
+  descend; step auto_ext.
+  2: returnScalar.
+  simpl.
+  make_toArray ("self" :: nil).
+  step auto_ext.
+  etransitivity; [ | apply (@is_state_in x2) ].
+  unfolder.
+  etransitivity; [ | apply himp_star_frame; [ reflexivity | apply is_heap_eat ] ].
+  do_delegate2 ("self" :: nil).
+
+  (* pop *)
+
+  do_abort ("self" :: nil).
+  do_abort ("self" :: nil).
+  do_abort ("self" :: nil).
+
+  do_delegate1 ("self" :: nil) hints.
+  repeat (apply andL || (apply injL; intro) || (apply existsL; intro)); reduce.
+  apply get_rval; intro.
+  descend; step auto_ext.
+  descend; step auto_ext.
+  2: returnScalar.
+  simpl.
+  make_toArray ("self" :: nil).
+  step auto_ext.
+  etransitivity; [ | apply (@is_state_in x2) ].
+  unfolder.
+  etransitivity; [ | apply himp_star_frame; [ reflexivity | apply readd_List ] ].
+  do_delegate2 ("self" :: nil).
+
+  (* empty *)
+
+  do_abort ("self" :: nil).
+  do_abort ("self" :: nil).
+  do_abort ("self" :: nil).
+
+  do_delegate1 ("self" :: nil) hints.
+  repeat (apply andL || (apply injL; intro) || (apply existsL; intro)); reduce.
+  apply get_rval; intro.
+  step auto_ext.
+  descend; step auto_ext.
+  2: returnScalar.
+  simpl.
+  make_toArray ("self" :: nil).
+  step auto_ext.
+  etransitivity; [ | apply (@is_state_in x2) ].
+  unfolder.
+  etransitivity; [ | apply himp_star_frame; [ reflexivity | apply readd_List ] ].
+  do_delegate2 ("self" :: nil).
+
+  (* push *)
+
+  do_abort ("self" :: "n" :: nil).
+  do_abort ("self" :: "n" :: nil).
+  do_abort ("self" :: "n" :: nil).
+
+  do_delegate1 ("self" :: "n" :: nil) hints.
+  add_side_conditions.
+  descend; step hints.
+  simpl.
+  descend; step auto_ext.
+  descend; step auto_ext.
+  simpl.
+  repeat (apply andL || (apply injL; intro) || (apply existsL; intro)); reduce.
+  apply get_rval; intro.
+  descend; step auto_ext.
+  2: returnScalar.
+  simpl.
+  make_toArray ("self" :: "n" :: nil).
+  step auto_ext.
+  etransitivity; [ | apply (@is_state_in x2) ].
+  unfolder.
+  etransitivity; [ | apply himp_star_frame; [ reflexivity | apply readd_List ] ].
+  do_delegate2 ("self" :: "n" :: nil).
+
+  (* copy *)
+
+  do_abort ("self" :: nil).
+  do_abort ("self" :: nil).
+  do_abort ("self" :: nil).
+
+  do_delegate1 ("self" :: nil) hints.
+  descend; step hints.
+  simpl.
+  descend; step auto_ext.
+  2: returnAdt.
+  simpl.
+  make_toArray ("self" :: nil).
+  step auto_ext.
+  etransitivity; [ | apply (@is_state_in x2) ].
+  unfolder.
+  etransitivity; [ | apply himp_star_frame; [ reflexivity | apply readd_List ] ].
+  do_delegate2 ("self" :: nil).
+
+
   Grab Existential Variables.
+  exact 0.
+  exact 0.
+  exact 0.
   exact 0.
   exact 0.
   exact 0.
@@ -306,12 +473,17 @@ Theorem ok0 : moduleOk m0.
 Qed.
 
 Definition m1 := link ListSetF.m m0.
-Definition m := link Malloc.m m1.
+Definition m2 := link ListSeqF.m m1.
+Definition m := link Malloc.m m2.
 
 Theorem ok1 : moduleOk m1.
   link ListSetF.ok ok0.
 Qed.
 
+Theorem ok2 : moduleOk m2.
+  link ListSeqF.ok ok1.
+Qed.
+
 Theorem ok : moduleOk m.
-  link Malloc.ok ok1.
+  link Malloc.ok ok2.
 Qed.
