platform/facade/examples/FiatRepInv.v
@@ -5,11 +5,11 @@ Require Import FiatADTs.
 Import Adt.
 Require Import Cito.RepInv.
 
-Require Import FiniteSetF ListSetF.
+Require Import FiniteSetF ListSetF SeqF ListSeqF.
 
 Definition rep_inv p adtvalue : HProp :=
   match adtvalue with
-    | List _ => [| False |]
+    | List ls => lseq ls p
     | Junk _ => [| False |]
     | FEnsemble s => lset s p
   end%Sep.
@@ -22,7 +22,7 @@ Module Ri <: RepInv FiatADTs.Adt.
 
   Lemma rep_inv_ptr : forall p a, rep_inv p a ===> p =?> 1 * any.
     destruct a; simpl.
-    sepLemma.
+    eapply Himp_trans; [ apply lseq_fwd | sepLemma ]; apply any_easy.
     sepLemma.
     eapply Himp_trans; [ apply lset_fwd | sepLemma ]; apply any_easy.
   Qed.
